verified/entry.i.dfy
@@ -139,7 +139,7 @@ predicate PrivKomUserEntryPrecondition(s:state, pagedb:PageDb, dispPg:PageNr)
     && s.conf.scr == SCRT(Secure, true, true)
     && StackBytesRemaining(s, EXCEPTION_STACK_BYTES)
     && validPageDb(pagedb) && pageDbCorresponds(s.m, pagedb)
-    && nonStoppedDispatcher(pagedb, dispPg)
+    && finalDispatcher(pagedb, dispPg)
     && GlobalWord(s.m, CurDispatcherOp(), 0) == page_monvaddr(dispPg)
     && s.conf.ttbr0.ptbase == page_paddr(l1pOfDispatcher(pagedb, dispPg))    
     && mode_of_state(s) != User
